\section{Quadratic Equations}

The quadratic equation 
\begin{equation}
\label{quad}
ax^2+bx+c = 0
\end{equation}

where \(a,b\) and \(c\) are constants and \(a \neq 0\), has two solutions for the variable \(x\):

\begin{equation}
\label{root}
x_{\alpha,\beta} = \frac{-b \pm \sqrt{b^2 - 4ac}}{2a}
\end{equation}

If the \emph{discriminant} \( \Delta \) with 

\begin{equation}
\label{delta}
\Delta = b^2 - 4ac = 0
\end{equation}

then the equation (\ref{quad}) has real and equal roots given by:

\begin{equation}
\label{equal_root}
x = \frac{-b}{2a}
\end{equation}

\textbf{Sum of the roots}:
\begin{equation}
\label{sum_root}
\alpha + \beta = \frac{-b}{a}
\end{equation}

\textbf{Product of the roots}:
\begin{equation}
\label{product_root}
\alpha.\beta = \frac{c}{a}
\end{equation}

\subsection{Factorization method}
Find the two factors $x-\alpha$ and $x-\beta$ which when multiplied produce the quadratic equation $ax^2+bx+c$. 

\subsection{Completion of squares method}
Consider any quadratic equation of the form $ax^2+bx+c = 0$. Dividing throughout by a.
\begin{align*}
\implies x^2+ \left(\frac{b}{a}\right) x +\frac{c}{a} &=0\\
\text{Adding and subtracting} &\left(\frac{b}{2a}\right)^{2}&,\\
x^2 + \left(\frac{b}{a}\right)x + \left(\frac{b}{2a}\right)^{2} - \left(\frac{b}{2a}\right)^{2} + \frac{c}{a} &=0\\
\end{align*}

\vspace{-10mm}

\begin{align*}
\left(x + \frac{b}{2a} \right)^{2} + \frac{c}{a} - \left(\frac{b}{2a}\right)^{2} &=0\\
\therefore ax^2+bx+c = 0 \implies a(x+d)^{2} + e &=0 \quad \text{where},\quad
d =\frac{b}{2a} \quad \text{and} \quad e = \frac{c}{a} - \left(\frac{b}{2a}\right)^{2}.
\end{align*}

\begin{center}
\textbf{***********}
\end{center}