\section{Basic Algebra}

\begin{equation}
\label{(a+b)2}
(a+b)^2 = a^2 + 2ab + b^2
\end{equation}

\begin{equation}
\label{(a-b)2}
(a-b)^2 = a^2 - 2ab + b^2
\end{equation}

\begin{equation}
\label{(a+b)(a-b)}
(a+b)(a-b) = a^2 - b^2
\end{equation}

\begin{equation}
\label{(a+b)3}
(a+b)^3 = a^3 + 3a^2b + 3ab^2 + b^3 = a^3 + b^3 + 3ab(a+b)
\end{equation}

\begin{equation}
\label{(a-b)3}
(a-b)^3 = a^3 - 3a^2b + 3ab^2 - b^3 = a^3 - b^3 - 3ab(a-b) 
\end{equation}

\begin{equation}
\label{a3+b3}
a^3+b^3 = (a+b)(a^2-ab+b^2) 
\end{equation}

\begin{equation}
\label{a3-b3}
a^3-b^3 = (a-b)(a^2+ab+b^2) 
\end{equation}

\begin{equation}
\label{a4-b4}
a^4-b^4 = (a+b)(a-b)(a^2+b^2) 
\end{equation}

\begin{equation}
\label{a2+b2}
a^2+b^2 = (a+b)^2 - 2ab 
\end{equation}

\begin{equation}
\label{a3+b3+c3}
a^3+b^3+c^3 - 3abc = (a+b+c)(a^2+b^2+c^2-ab-bc-ac)
\end{equation}