\section{Permutations and Combinations}
%\begin{equation}
\begin{align}
\binom{n}{r} &= \frac{n!}{r!(n-r)!} = \frac{n(n-1)(n-2)(n-3).....(n-(r+1))}{r!}
\end{align} \\

Note that:
\begin{align*}
\binom{n}{0} &= 1  &  \binom{n}{1} &= n  &  0! &= 1
\end{align*}

\subsection{Binomial Theorem}
\begin{align}
(x+a)^{n} = x^{n} + \binom{n}{1} x^{n-1}a + \binom{n}{2} x^{n-2}a^2 +  \binom{n}{3} x^{n-3}a^3 +  \binom{n}{4} x^{n-4}a^4 + ............ a^n
\end{align}

\subsection{Summation of Series}
\begin{align}
\sum_{n=1}^{\infty} n &= 1+2+3...... = \frac{(n)(n+1)}{2} \\
\sum_{n=1}^{\infty} n^2 &= 1^2+2^2+3^2...... = \frac{(n)(n+1)(2n+1)}{6}\\
\sum_{n=1}^{\infty} n^3 &= 1^3+2^3+3^3...... = \frac{(n)^{2}(n+1)^2}{4}
\end{align}

\vspace{5mm}
\begin{center}
\textbf{***********}
\end{center}